projects/lib/gmp_goal_check.v
@@ -1,6 +1,6 @@
-From  Require Import gmp_goal gmp_proof_auto gmp_proof_manual.
+From  Require Import gmp_goal gmp_proof_auto gmp_proof_manual_tmp.
 
 Module VC_Correctness : VC_Correct.
   Include gmp_proof_auto.
-  Include gmp_proof_manual.
+  Include gmp_proof_manual_tmp.
 End VC_Correctness.
